src/goose_lang/spec_assert.v
@@ -28,9 +28,9 @@ Context {spec_ffi_semantics: spec_ext_semantics spec_ext spec_ffi}.
 Context `{!spec_ffi_interp spec_ffi}.
 
 Canonical Structure spec_lang : language :=
-  @heap_lang (spec_ext_op_field) (spec_ffi_model_field) (spec_ext_semantics_field).
+  @goose_lang (spec_ext_op_field) (spec_ffi_model_field) (spec_ext_semantics_field).
 Canonical Structure spec_crash_lang : crash_semantics spec_lang :=
-  @heap_crash_lang (spec_ext_op_field) (spec_ffi_model_field) (spec_ext_semantics_field).
+  @goose_crash_lang (spec_ext_op_field) (spec_ffi_model_field) (spec_ext_semantics_field).
 
 Existing Instance spec_ffi_interp_field.
 Existing Instance spec_ext_semantics_field.
